changed TSB definition to allow uneq tickcount

TSB.thy
@@ -1,15 +1,16 @@
 (*  Title:        TSBTheorie.thy
-    Author:       Sebastian Stüber
-    e-mail:       sebastian.stueber@rwth-aachen.de
+    Author:       Sebastian Stüber, Jens Christoph Bürger
+    e-mail:       sebastian.stueber@rwth-aachen.de,
+                  jens.buerger@rwth-aachen.de
 
     Description:  Definition of "Timed Stream Bundles"
-                    in 3 different versions, a general "TSB"  
+                    in 3 different versions, a general "TSB"
                                              one over infinite TStreams "TSB_inf"
                                              and one over finite TStreams "TSB_fin"
 *)
 
 
-chapter {* Timed Streams *} 
+chapter {* Timed Streams *}
 
 theory TSB
 imports Channel OptionCpo TStream TStream_JB
@@ -18,7 +19,7 @@ begin
 
 
 default_sort message
-  
+
 
 (* ----------------------------------------------------------------------- *)
   section \<open>TSB\<close>
@@ -27,66 +28,36 @@ default_sort message
  (* Definition: Welltyped. "a \<rightharpoonup> b" means "a => b option" *)
   (* Every TStream may only contain certain elements *)
   (* and alle tstreams must have the same number of \<surd> *)
-definition tsb_well :: "(channel \<rightharpoonup> 'm tstream) => bool" where
-"tsb_well f \<equiv> (\<forall>c \<in> dom f. tsDom\<cdot>(f\<rightharpoonup>c) \<subseteq> ctype c) 
-        \<and> (\<exists>n. \<forall>c \<in> dom f.  #\<surd>(f\<rightharpoonup>c) = n)"
-
-lemma tstick_count_help: assumes "chain Y" and "\<not>finite_chain Y" 
-    and "\<And>i. \<exists>n. \<forall>c \<in> dom (Y i). #\<surd>((Y i)\<rightharpoonup>c) = n" and "c\<in>dom (Y 0)"
-  shows "\<not>finite_chain (\<lambda>i. ((Y i) \<rightharpoonup> c))"
-proof(rule ccontr, simp)
-  assume fin_y: "finite_chain (\<lambda>i. (Y i)\<rightharpoonup>c)"
-  hence ch_y: "chain (\<lambda>i. (Y i)\<rightharpoonup>c)" using finite_chain_def by blast
-  obtain j where j_def: "max_in_chain j (\<lambda>i. (Y i)\<rightharpoonup>c)" using fin_y finite_chainE by auto
-  hence "\<And>c2. c2\<in>dom (Y 0) \<Longrightarrow>  max_in_chain j (\<lambda>i. (Y i)\<rightharpoonup>c2)" 
-  proof -
-    fix c2
-    assume c2_as: "c2\<in>dom (Y 0)" 
-    hence c2_dom: "\<And>i. c2\<in>dom (Y i)" using assms(1) part_dom_eq1 by blast
-    hence "\<And>i. #\<surd> (Y i)\<rightharpoonup>c = #\<surd>(Y i)\<rightharpoonup>c2" by (metis assms(1) assms(3) assms(4) part_dom_eq1)
-    hence f1: "\<And>i. j\<le>i \<Longrightarrow> #\<surd>(Y i)\<rightharpoonup>c2 =  #\<surd> (Y j)\<rightharpoonup>c2" by (metis j_def max_in_chainD)
-    hence "\<And>i. j\<le>i \<Longrightarrow> (Y j)\<rightharpoonup>c2 \<sqsubseteq> (Y i)\<rightharpoonup>c2" by (metis assms(1) part_the_chain po_class.chain_mono)
-    hence "\<And>i. j\<le>i \<Longrightarrow> (Y i)\<rightharpoonup>c2 =  (Y j)\<rightharpoonup>c2" using local.f1 tstake_below_eq by fastforce 
-    thus "max_in_chain j (\<lambda>i. (Y i)\<rightharpoonup>c2)" by (metis (no_types, lifting) max_in_chainI)
-  qed 
-  hence "max_in_chain j Y" by (metis (no_types, lifting) assms(1) max_in_chainD max_in_chainI part_dom_eq1 part_eq) 
-  thus False using assms(1) assms(2) finite_chainl1 by blast 
-qed
-
-
-(* checking whether every stream in the range of a partial function f has the same number of ticks 
-   is an admissible predicate *)
-lemma tstick_count_adm: "adm (\<lambda> f. \<exists>n. \<forall>c::channel \<in> dom f. #\<surd>(f\<rightharpoonup>c) = n)"
-  apply(rule admI)
-  apply(rename_tac Y)
-  apply (case_tac "finite_chain Y \<or> dom (\<Squnion>i. Y i) = {}")
-   apply (metis equals0D l42)
-  by (metis (mono_tags, lifting) part_dom_lub part_the_chain part_the_lub ts_infinite_lub tstick_count_help)
+definition tsb_well :: "(channel \<rightharpoonup> 'm tstream) \<Rightarrow> bool" where
+"tsb_well f \<equiv> (\<forall>c \<in> dom f. tsDom\<cdot>(f\<rightharpoonup>c) \<subseteq> ctype c)"
 
 
 lemma tsb_welltyped_adm [simp]: "adm (\<lambda>f. \<forall>c \<in> dom f. tsDom\<cdot>(f\<rightharpoonup>c) \<subseteq> ctype c)"
   by (simp add: adm_def lub_fun part_dom_lub the_subset_cont)
 
-
 lemma tsb_well_adm [simp]: "adm (\<lambda>f. tsb_well f)"
-  apply(subst tsb_well_def)
-  apply (rule adm_conj)
-   using tsb_welltyped_adm apply blast
-  by (simp add: tstick_count_adm)
+  apply (subst tsb_well_def)
+   using tsb_welltyped_adm by blast
 
+lemma tsb_well_exists [simp]: "tsb_well empty"
+  by (simp add: tsb_well_def)
 
 (* Definition: Timed Stream Bundle. *)
 cpodef 'm :: message TSB = "{b :: channel \<rightharpoonup> 'm tstream . tsb_well b }"
    using tsb_well_def apply fastforce
-  by auto
+   by auto
 
 setup_lifting type_definition_TSB
 
 
-
   subsection \<open>Definitions on TSB \<close>
 (* ----------------------------------------------------------------------- *)
-
+    
+(* Syntactic sugar for Abs_TSB *)
+abbreviation Abs_abbr :: "(channel \<rightharpoonup> 'm tstream) \<Rightarrow> 'm TSB" ("_\<Omega>" [65] 65) where 
+"f \<Omega> \<equiv> Abs_TSB f"
+    
+text \<open>@{text "tsbDom"} returns the domain of the timed stream bundle\<close>
 definition tsbDom :: "'m TSB \<rightarrow> channel set" where
 "tsbDom \<equiv> \<Lambda> tb. dom (Rep_TSB tb)"
 
@@ -94,70 +65,51 @@ definition TSB :: "channel set \<Rightarrow> 'm TSB set" where
 "TSB cs \<equiv> {b. tsbDom\<cdot>b = cs}"
 
 
-(* returns the tstream flowing in given channel *)
+text {* @{text "sbGetCh"} returns the tstream flowing on a channel of a timed stream bundle *}
 definition tsbGetCh :: "'m TSB \<rightarrow> channel \<rightarrow> 'm tstream" where
 "tsbGetCh \<equiv> \<Lambda> tb c. ((Rep_TSB tb) \<rightharpoonup> c)"
 
-abbreviation tsbGetCh_abbr :: "'m TSB \<Rightarrow> channel \<Rightarrow>  'm tstream" (infix " . " 65)
-where "b . c \<equiv> tsbGetCh\<cdot>b\<cdot>c"
+abbreviation tsbGetCh_abbr :: "'m TSB \<Rightarrow> channel \<Rightarrow>  'm tstream" (infix " . " 65) where 
+"b . c \<equiv> tsbGetCh\<cdot>b\<cdot>c"
+
+
+text {* For a given channel set, "tsbLeast" is the smallest stream bundle with empty tstreams. *}
+definition tsbLeast :: "channel set \<Rightarrow> 'm TSB" where
+"tsbLeast cs = Abs_TSB (optionLeast cs)"
+
+
+text {* @{text "tsbunion"} the channel-domains are merged *}
+definition tsbUnion :: "'m TSB \<rightarrow> 'm TSB \<rightarrow> 'm TSB"  where 
+"tsbUnion \<equiv> \<Lambda> tb1 tb2 . Abs_TSB ((Rep_TSB tb1) ++ (Rep_TSB tb2))"
+
+abbreviation tsbUnion_abbrv :: "'m TSB \<Rightarrow> 'm TSB \<Rightarrow> 'm TSB" (infixl "\<uplus>" 100) where
+"tb1 \<uplus> tb2 \<equiv> tsbUnion\<cdot>tb1\<cdot>tb2"
+
+
+text {* @{text "tsbsetch"} adds a channel or replaces its content *}
+definition tsbSetCh :: "'m TSB \<rightarrow> channel \<Rightarrow> 'm tstream \<Rightarrow> 'm TSB" where
+"tsbSetCh \<equiv> \<Lambda> b. (\<lambda> c s. b \<uplus> (Abs_TSB([c \<mapsto> s])))"
 
 
  (* Channels not in the channel set are set to "None". *)
 definition tsbRestrict:: "channel set \<Rightarrow> 'm TSB \<rightarrow> 'm TSB" where
 "tsbRestrict cs \<equiv>  \<Lambda> b. Abs_TSB (Rep_TSB b |` cs)"
 
-abbreviation tsbRestrict_abbr :: "'m TSB \<Rightarrow> channel set \<Rightarrow> 'm TSB" (infix "\<bar>" 65)
-where "b\<bar>cs \<equiv> tsbRestrict cs\<cdot>b"
+abbreviation tsbRestrict_abbr :: "'m TSB \<Rightarrow> channel set \<Rightarrow> 'm TSB" (infix "\<bar>" 65) where 
+"b\<bar>cs \<equiv> tsbRestrict cs\<cdot>b"
 
-  
+
 (* returns the first n blocks of the TSB *)
-definition tsbTTake :: "nat \<Rightarrow> 'm TSB \<Rightarrow> 'm TSB" where 
+definition tsbTTake :: "nat \<Rightarrow> 'm TSB \<Rightarrow> 'm TSB" where
 "tsbTTake n tb = Abs_TSB (\<lambda>c. (c\<in>tsbDom\<cdot>tb) \<leadsto> (tsTake n\<cdot>(tb  .  c)))"
-                                                 
+
 
 abbreviation tsbTTake_abbrv :: "'m TSB \<Rightarrow> nat \<Rightarrow> 'm TSB" ("_ \<down> _ ")where
 "tb \<down> n \<equiv> tsbTTake n tb"
 
 (* defintion with lnat *)
-definition tsbTTakeL :: "lnat \<Rightarrow> 'm TSB \<Rightarrow> 'm TSB" where 
+definition tsbTTakeL :: "lnat \<Rightarrow> 'm TSB \<Rightarrow> 'm TSB" where
 "tsbTTakeL n tb = Abs_TSB (\<lambda>c. (c\<in>tsbDom\<cdot>tb) \<leadsto> (tsTakeL\<cdot>n\<cdot>(tb  .  c)))"
-
-definition tsbLeast :: "channel set \<Rightarrow> 'm TSB" where 
-"tsbLeast cs = Abs_TSB (optionLeast cs)"
-
-
-
-
-
-
-
-
-definition tsbTickCount :: "'m TSB \<rightarrow> lnat" where
-"tsbTickCount \<equiv>  \<Lambda> tb. if tsbDom\<cdot>tb \<noteq> {} then #\<surd>(SOME ts. ts \<in> ran (Rep_TSB tb)) else \<infinity>"
-
-abbreviation tsbTickCount_abbrv :: "'m TSB \<Rightarrow> lnat "  ("#\<surd>tsb _ ") where
-" #\<surd>tsb tsb \<equiv> tsbTickCount\<cdot>tsb"
-
-
-definition tsbMinTick :: "'m TSB \<Rightarrow> 'm TSB \<Rightarrow> lnat" where
-"tsbMinTick tb1 tb2 \<equiv> lnmin\<cdot>(#\<surd>tsb tb1)\<cdot>(#\<surd>tsb tb2)"
-
-
-definition tsbUnion :: "'m TSB \<rightarrow> 'm TSB \<rightarrow> 'm TSB"  where 
-"tsbUnion \<equiv> \<Lambda> tb1 tb2 . let l1 = #\<surd>tsb tb1; l2 = #\<surd>tsb tb2  in 
-            Abs_TSB ((Rep_TSB (tsbTTakeL l2 tb1)) ++ (Rep_TSB (tsbTTakeL l1 tb2)))"
-
-abbreviation tsbUnion_abbrv :: "'m TSB \<Rightarrow> 'm TSB \<Rightarrow> 'm TSB" (infixl "\<uplus>" 100) where
-"tb1 \<uplus> tb2 \<equiv> tsbUnion\<cdot>tb1\<cdot>tb2"
-
-definition tsbUnion2 :: "'m TSB \<rightarrow> 'm TSB \<rightarrow> 'm TSB"  where 
-"tsbUnion2 \<equiv> \<Lambda> tb1 tb2 . Abs_TSB ((Rep_TSB tb1) ++ (Rep_TSB tb2))"
-
-(* NEW *)
-
-text {* @{text "tsbsetch"} adds a channel or replaces its content *}
-definition tsbSetCh :: "'m TSB \<rightarrow> channel \<Rightarrow> 'm tstream \<Rightarrow> 'm TSB" where
-"tsbSetCh \<equiv> \<Lambda> b. (\<lambda> c s. b \<uplus> (Abs_TSB([c \<mapsto> s])))"
 
 
 text {* @{text "tsbRemCh"} removes a channel from a timed stream bundle *}
@@ -166,11 +118,17 @@ abbreviation tsbRemCh :: "'m TSB \<rightarrow> channel \<rightarrow> 'm TSB" whe
 
 definition tsbRenameCh :: "'m TSB \<Rightarrow> channel \<Rightarrow> channel \<Rightarrow> 'm TSB" where
  "tsbRenameCh b ch1 ch2 \<equiv> (tsbSetCh\<cdot>(tsbRemCh\<cdot>b\<cdot>ch1)) ch2 (b . ch1)"
- 
- 
-(* sbUp not yet ported *)
- 
- 
+
+
+  (* Replaces all "None" channels with \<epsilon>. *)
+      (* untested *)
+definition tsbUp:: " 'm TSB \<rightarrow> 'm TSB"  where
+"tsbUp \<equiv> \<Lambda> b . Abs_TSB (\<lambda>c. if (c \<in> tsbDom\<cdot>b) then (Rep_TSB b) c else Some \<bottom>)"
+
+abbreviation tsbUp_abbr:: " 'm TSB \<Rightarrow> 'm TSB"  ("\<up>_" 70) where
+"\<up>b \<equiv> tsbUp\<cdot>b"
+
+
 text {* @{text "tsbeqch"} equality on specific channels *}
 definition tsbEqSelected:: " channel set \<Rightarrow> 'm TSB => 'm TSB => bool" where
 "tsbEqSelected cs b1 b2 \<equiv>  (b1\<bar>cs) = (b2\<bar>cs)"
@@ -182,11 +140,11 @@ definition tsbEqCommon:: " 'm TSB => 'm TSB => bool" where
 
 text {* @{text " tsbPrefixSelected"} prefix relation on selected channels *}
 definition tsbPrefixSelected:: "channel set \<Rightarrow> 'm TSB \<Rightarrow> 'm TSB \<Rightarrow> bool" where
-"tsbPrefixSelected cs b1 b2 \<equiv> (b1\<bar>cs \<sqsubseteq> b2\<bar>cs)" 
+"tsbPrefixSelected cs b1 b2 \<equiv> (b1\<bar>cs \<sqsubseteq> b2\<bar>cs)"
 
 text {* @{text " tsbPrefixCommon"} prefix relation on common channels *}
 definition tsbPrefixCommon:: " 'm TSB \<Rightarrow> 'm TSB \<Rightarrow> bool" where
-"tsbPrefixCommon b1 b2 \<equiv> tsbPrefixSelected (tsbDom\<cdot>b1 \<inter> tsbDom\<cdot>b2) b1 b2" 
+"tsbPrefixCommon b1 b2 \<equiv> tsbPrefixSelected (tsbDom\<cdot>b1 \<inter> tsbDom\<cdot>b2) b1 b2"
 
 
 (* sbConc not yet ported *)
@@ -221,14 +179,15 @@ definition tsbNth:: "nat \<Rightarrow> 'm TSB \<Rightarrow> 'm TSB" where
 
 
 lemma rep_tsb_cont [simp]: "cont Rep_TSB"
-  by (smt Abs_TSB_inverse adm_TSB adm_def below_TSB_def contI lub_TSB lub_eq po_class.chain_def thelubE type_definition.Rep type_definition_TSB)
+  by (smt Abs_TSB_inverse adm_TSB adm_def below_TSB_def contI lub_TSB lub_eq po_class.chain_def 
+          thelubE type_definition.Rep type_definition_TSB)
 
 lemma rep_chain[simp]: assumes "chain S"
   shows "chain (\<lambda>n. Rep_TSB (S n))"
   by (meson assms below_TSB_def po_class.chain_def)
 
 text {* Equivalence of evaluation of StBundleLub based on lub of function values.*}
-lemma lub_eval: assumes "chain S" 
+lemma lub_eval: assumes "chain S"
   shows "the (Rep_TSB (\<Squnion>i. S i) c) = (\<Squnion>j. the (Rep_TSB (S j) c))"
 proof -
   have f1: "Rep_TSB (Lub S) = (\<Squnion>n. Rep_TSB (S n))"
@@ -241,7 +200,7 @@ proof -
     using f1 by (metis (no_types) part_the_lub)
 qed
 
-lemma theRep_chain[simp]: assumes "chain S" 
+lemma theRep_chain[simp]: assumes "chain S"
   shows "chain (\<lambda>n. the (Rep_TSB (S n) c))"
   using assms part_the_chain rep_chain by fastforce
 
@@ -265,33 +224,33 @@ lemma [simp]: "Abs_TSB (Rep_TSB y) = y"
   by (simp add: Rep_TSB_inverse)
 
 lemma [simp]: "tsb_well empty"
-  by(simp add: tsb_well_def)
+  by (simp add: tsb_well_def)
 
+    (* obsolete
 lemma ts_ex_len [simp]: "\<exists> ln . ( \<forall> c . (c \<in> (dom (Rep_TSB b)) \<longrightarrow> ((#\<surd> ((Rep_TSB b) \<rightharpoonup> c)) = ln)))"
   using Rep_TSB tsb_well_def  using mem_Collect_eq by force
+*)
 
 lemma [simp]: assumes "tsb_well f" and "c\<in>dom f"
   shows "tsDom\<cdot>f\<rightharpoonup>c \<subseteq> ctype c"
   using assms(1) assms(2) tsb_well_def by blast
 
+    (* obsolete
 lemma tsb_tick_eq: assumes "tsb_well f" and "c1\<in>dom f" and "c2\<in>dom f"
   shows "#\<surd> f\<rightharpoonup>c1 = #\<surd> f\<rightharpoonup>c2"
   by (metis assms(1) assms(2) assms(3) tsb_well_def)
+*)
 
-
-lemma tsb_wellI: 
-  assumes "\<And> c. c\<in>dom f \<Longrightarrow> tsDom\<cdot>f\<rightharpoonup>c \<subseteq> ctype c"
-  and "\<exists>ln. (\<forall> c. c\<in>dom f \<longrightarrow>  #\<surd> f\<rightharpoonup>c = ln)"
+lemma tsb_wellI: assumes "\<And> c. c\<in>dom f \<Longrightarrow> tsDom\<cdot>f\<rightharpoonup>c \<subseteq> ctype c"
   shows "tsb_well f"
-  apply(simp add: tsb_well_def assms)
-  using assms(2) by blast
+  using assms(1) tsb_well_def by blast
 
 
 
 
 
 subsubsection \<open>tsbDom\<close>
-  
+
 thm tsbDom_def
 
 
@@ -302,13 +261,13 @@ lemma tsbdom_insert: "tsbDom\<cdot>tb = dom (Rep_TSB tb)"
   by (simp add: tsbDom_def)
 
 lemma tsbdom_rep_eq: "tsb_well tb \<Longrightarrow> tsbDom\<cdot>(Abs_TSB tb) = dom tb"
-by(simp add: tsbdom_insert)
+by (simp add: tsbdom_insert)
 
 
 lemma tsbdom_below: assumes "tb1 \<sqsubseteq> tb2"
   shows "tsbDom\<cdot>tb1 = tsbDom\<cdot>tb2"
   by (metis assms below_TSB_def part_dom_eq tsbdom_insert)
-    
+
 lemma tsbChain_dom_eq3: assumes "chain S"
   shows "tsbDom\<cdot>(S i) = tsbDom\<cdot>(S j)"
   using assms is_ub_thelub tsbdom_below by blast
@@ -319,7 +278,7 @@ lemma tsbChain_dom_eq2[simp]: assumes "chain S"
 
 lemma tsdom_ctype_subset[simp]: assumes "c\<in>tsbDom\<cdot>tsb"
   shows "tsDom\<cdot>(Rep_TSB tsb)\<rightharpoonup>c \<subseteq> ctype c"
-  using assms by(simp add: tsbdom_insert)
+  using assms by (simp add: tsbdom_insert)
 
 lemma tsbdom_lub: assumes "chain Y" and "tsbDom\<cdot>(Y i) = cs"
   shows "tsbDom\<cdot>(\<Squnion> i. Y i) = cs"
@@ -328,7 +287,7 @@ lemma tsbdom_lub: assumes "chain Y" and "tsbDom\<cdot>(Y i) = cs"
 
 
 subsubsection \<open>tsbGetCh\<close>
-  
+
 thm tsbGetCh_def
 
 lemma tsbgetch_cont1 [simp]: "cont (\<lambda>tb  c . ((Rep_TSB tb) \<rightharpoonup> c))"
@@ -339,28 +298,23 @@ using cont2cont_LAM_discrete cont2cont_fun by force
 
 
 lemma tsbgetch_insert: "tsb  .  c = (Rep_TSB tsb) \<rightharpoonup> c"
-by(simp add: tsbGetCh_def)
+by (simp add: tsbGetCh_def)
 
 lemma tsbgetch_rep_eq: "tsb_well tb \<Longrightarrow> (Abs_TSB tb) . c = tb\<rightharpoonup>c"
-by(simp add: tsbgetch_insert)
+by (simp add: tsbgetch_insert)
 
 
 lemma tsbgetchE: assumes "c \<in> tsbDom\<cdot>tsb"
   shows "Some (tsb . c) = (Rep_TSB tsb) c"
-  by (metis assms domD is_none_code(2) is_none_simps(1) option.collapse tsbdom_insert 
+  by (metis assms domD is_none_code(2) is_none_simps(1) option.collapse tsbdom_insert
             tsbgetch_insert)
-  
+
 lemma lubgetCh: assumes "chain Y" and "c \<in> tsbDom\<cdot>(\<Squnion> i. Y i)"
   shows "(\<Squnion>i. Y i) . c = (\<Squnion>i. (Y i) . c)"
   by (simp add: assms(1) contlub_cfun_arg contlub_cfun_fun)
-          
-          
-subsubsection \<open>eq/below\<close>  
-  
-lemma tsb_tick_eq2: assumes "c1\<in>tsbDom\<cdot>f" and "c2\<in>tsbDom\<cdot>f"
-  shows "#\<surd> f . c1 = #\<surd> f . c2"
-  using assms by(simp add: tsbdom_insert tsbgetch_insert tsb_tick_eq)
 
+
+subsubsection \<open>eq/below\<close>
 
 lemma tsb_below: assumes "tsbDom\<cdot>x = tsbDom\<cdot>y" and "\<And> c. c\<in>tsbDom\<cdot>x \<Longrightarrow> x . c \<sqsubseteq>y . c"
   shows "x\<sqsubseteq>y"
@@ -374,22 +328,23 @@ lemma tsb_eq: assumes "tsbDom\<cdot>x = tsbDom\<cdot>y" and "\<And> c. c\<in>tsb
 lemma tsbgetch_eq2: "b = Abs_TSB(\<lambda> c. (c \<in> tsbDom\<cdot>b) \<leadsto> b . c)"
   apply (rule tsb_eq)
    apply (subst tsbdom_rep_eq)
-    apply (smt Collect_cong Rep_TSB dom_def mem_Collect_eq option.collapse part_eq tsbdom_insert tsbgetch_insert)
+    apply (smt Collect_cong Rep_TSB dom_def mem_Collect_eq option.collapse part_eq tsbdom_insert 
+               tsbgetch_insert)
     apply (simp)
     by (smt Collect_cong Rep_TSB_inverse dom_def mem_Collect_eq part_eq tsbdom_insert tsbgetchE)
-    
+
 
 subsubsection \<open>tsbLeast\<close>
-  
+
 lemma tsbleast_well [simp]: "tsb_well (optionLeast cs)"
-  by(simp add: tsb_well_def)
+  by (simp add: tsb_well_def)
 
 lemma tsbleast_tsdom [simp]: "tsbDom\<cdot>(tsbLeast cs) = cs"
-  by(simp add: tsbLeast_def tsbDom_def)
+  by (simp add: tsbLeast_def tsbDom_def)
 
 lemma tsbleast_getch[simp]:  assumes "c\<in>cs"
   shows "tsbLeast cs  .  c = \<bottom>"
-  by(simp add: tsbLeast_def tsbgetch_insert assms)
+  by (simp add: tsbLeast_def tsbgetch_insert assms)
 
 lemma tsbleast_below [simp]: assumes "cs = tsbDom\<cdot>b"
   shows "tsbLeast cs \<sqsubseteq> b"
@@ -400,13 +355,13 @@ proof -
     apply (subst tsb_below)
     by (simp_all add: assms)
 qed
-  
 
-  
+
+
 
 
 subsubsection \<open>TSB\<close>
-    
+
 lemma tsb_tsbleast [simp]:  "tsbLeast cs \<in> TSB cs"
   by (simp add: TSB_def)
 
@@ -424,31 +379,63 @@ thm tsbRestrict_def
 
 
 lemma tsbrestrict_well[simp] : "tsb_well (Rep_TSB b |` cs)"
-  apply(rule tsb_wellI)
-   apply (metis Rep_TSB domIff mem_Collect_eq restrict_in restrict_out tsb_well_def)
-  by (metis Int_iff dom_restrict restrict_in ts_ex_len)
+  apply (rule tsb_wellI)
+  by auto
+  
 
 
 lemma tsbrestrict_monofun[simp]: "monofun  (\<lambda>b. Rep_TSB b |` cs)"
 proof -
-  have "\<forall>f. (\<exists>t ta. (t::'a TSB) \<sqsubseteq> ta \<and> (f t::channel \<Rightarrow> 'a tstream option) \<notsqsubseteq> f ta) \<or> monofun f"
+  have "\<forall>f. (\<exists>t ta. (t::'a TSB) \<sqsubseteq> ta 
+                    \<and> (f t::channel \<Rightarrow> 'a tstream option) \<notsqsubseteq> f ta) \<or> monofun f"
     using monofunI by blast
-  then obtain tt :: "('a TSB \<Rightarrow> channel \<Rightarrow> 'a tstream option) \<Rightarrow> 'a TSB" and tta :: "('a TSB \<Rightarrow> channel \<Rightarrow> 'a tstream option) \<Rightarrow> 'a TSB" where
+  then obtain tt :: "('a TSB \<Rightarrow> channel \<Rightarrow> 'a tstream option) \<Rightarrow> 'a TSB" 
+        and tta :: "('a TSB \<Rightarrow> channel \<Rightarrow> 'a tstream option) \<Rightarrow> 'a TSB" where
     f1: "\<forall>f. tt f \<sqsubseteq> tta f \<and> f (tt f) \<notsqsubseteq> f (tta f) \<or> monofun f"
     by (metis (no_types))
   obtain cc :: "(channel \<Rightarrow> 'a tstream option) \<Rightarrow> (channel \<Rightarrow> 'a tstream option) \<Rightarrow> channel" where
         "\<forall>x0 x1. (\<exists>v2. x1 v2 \<notsqsubseteq> x0 v2) = (x1 (cc x0 x1) \<notsqsubseteq> x0 (cc x0 x1))"
     by moura
-  then have f2: "\<forall>f fa. (f \<notsqsubseteq> fa \<or> (\<forall>c. f c \<sqsubseteq> fa c)) \<and> (f \<sqsubseteq> fa \<or> f (cc fa f) \<notsqsubseteq> fa (cc fa f))"
+  then have f2: "\<forall>f fa. (f \<notsqsubseteq> fa \<or> (\<forall>c. f c \<sqsubseteq> fa c)) 
+                        \<and> (f \<sqsubseteq> fa \<or> f (cc fa f) \<notsqsubseteq> fa (cc fa f))"
     by (metis fun_below_iff)
-  then have f3: "(Rep_TSB (tt (\<lambda>t. Rep_TSB t |` cs)) |` cs \<notsqsubseteq> Rep_TSB (tta (\<lambda>t. Rep_TSB t |` cs)) |` cs \<or> (\<forall>c. (Rep_TSB (tt (\<lambda>t. Rep_TSB t |` cs)) |` cs) c \<sqsubseteq> (Rep_TSB (tta (\<lambda>t. Rep_TSB t |` cs)) |` cs) c)) \<and> (Rep_TSB (tt (\<lambda>t. Rep_TSB t |` cs)) |` cs \<sqsubseteq> Rep_TSB (tta (\<lambda>t. Rep_TSB t |` cs)) |` cs \<or> (Rep_TSB (tt (\<lambda>t. Rep_TSB t |` cs)) |` cs) (cc (Rep_TSB (tta (\<lambda>t. Rep_TSB t |` cs)) |` cs) (Rep_TSB (tt (\<lambda>t. Rep_TSB t |` cs)) |` cs)) \<notsqsubseteq> (Rep_TSB (tta (\<lambda>t. Rep_TSB t |` cs)) |` cs) (cc (Rep_TSB (tta (\<lambda>t. Rep_TSB t |` cs)) |` cs) (Rep_TSB (tt (\<lambda>t. Rep_TSB t |` cs)) |` cs)))"
+  then have f3: "(Rep_TSB (tt (\<lambda>t. Rep_TSB t |` cs)) |` cs \<notsqsubseteq> 
+                  Rep_TSB (tta (\<lambda>t. Rep_TSB t |` cs)) |` cs 
+                    \<or> (\<forall>c. (Rep_TSB (tt (\<lambda>t. Rep_TSB t |` cs)) |` cs) c 
+                    \<sqsubseteq> (Rep_TSB (tta (\<lambda>t. Rep_TSB t |` cs)) |` cs) c)) 
+                    \<and> (Rep_TSB (tt (\<lambda>t. Rep_TSB t |` cs)) |` cs 
+                    \<sqsubseteq> Rep_TSB (tta (\<lambda>t. Rep_TSB t |` cs)) |` cs 
+                    \<or> (Rep_TSB (tt (\<lambda>t. Rep_TSB t |` cs)) |` cs) 
+                      (cc (Rep_TSB (tta (\<lambda>t. Rep_TSB t |` cs)) |` cs) 
+                      (Rep_TSB (tt (\<lambda>t. Rep_TSB t |` cs)) |` cs)) \<notsqsubseteq> 
+                      (Rep_TSB (tta (\<lambda>t. Rep_TSB t |` cs)) |` cs) 
+                      (cc (Rep_TSB (tta (\<lambda>t. Rep_TSB t |` cs)) |` cs) 
+                      (Rep_TSB (tt (\<lambda>t. Rep_TSB t |` cs)) |` cs)))"
     by blast
-  { assume "Rep_TSB (tt (\<lambda>t. Rep_TSB t |` cs)) (cc (Rep_TSB (tta (\<lambda>t. Rep_TSB t |` cs)) |` cs) (Rep_TSB (tt (\<lambda>t. Rep_TSB t |` cs)) |` cs)) \<sqsubseteq> Rep_TSB (tta (\<lambda>t. Rep_TSB t |` cs)) (cc (Rep_TSB (tta (\<lambda>t. Rep_TSB t |` cs)) |` cs) (Rep_TSB (tt (\<lambda>t. Rep_TSB t |` cs)) |` cs))"
+  { assume "Rep_TSB (tt (\<lambda>t. Rep_TSB t |` cs)) (cc (Rep_TSB (tta (\<lambda>t. Rep_TSB t |` cs)) |` cs) 
+             (Rep_TSB (tt (\<lambda>t. Rep_TSB t |` cs)) |` cs)) \<sqsubseteq> Rep_TSB (tta (\<lambda>t. Rep_TSB t |` cs)) 
+              (cc (Rep_TSB (tta (\<lambda>t. Rep_TSB t |` cs)) |` cs) 
+                (Rep_TSB (tt (\<lambda>t. Rep_TSB t |` cs)) |` cs))"
     moreover
-    { assume "(Rep_TSB (tt (\<lambda>t. Rep_TSB t |` cs)) (cc (Rep_TSB (tta (\<lambda>t. Rep_TSB t |` cs)) |` cs) (Rep_TSB (tt (\<lambda>t. Rep_TSB t |` cs)) |` cs)) \<sqsubseteq> Rep_TSB (tta (\<lambda>t. Rep_TSB t |` cs)) (cc (Rep_TSB (tta (\<lambda>t. Rep_TSB t |` cs)) |` cs) (Rep_TSB (tt (\<lambda>t. Rep_TSB t |` cs)) |` cs))) \<noteq> ((Rep_TSB (tt (\<lambda>t. Rep_TSB t |` cs)) |` cs) (cc (Rep_TSB (tta (\<lambda>t. Rep_TSB t |` cs)) |` cs) (Rep_TSB (tt (\<lambda>t. Rep_TSB t |` cs)) |` cs)) \<sqsubseteq> (Rep_TSB (tta (\<lambda>t. Rep_TSB t |` cs)) |` cs) (cc (Rep_TSB (tta (\<lambda>t. Rep_TSB t |` cs)) |` cs) (Rep_TSB (tt (\<lambda>t. Rep_TSB t |` cs)) |` cs)))"
-      then have "cc (Rep_TSB (tta (\<lambda>t. Rep_TSB t |` cs)) |` cs) (Rep_TSB (tt (\<lambda>t. Rep_TSB t |` cs)) |` cs) \<notin> cs"
+    { assume "(Rep_TSB (tt (\<lambda>t. Rep_TSB t |` cs)) (cc (Rep_TSB (tta (\<lambda>t. Rep_TSB t |` cs)) |` cs) 
+              (Rep_TSB (tt (\<lambda>t. Rep_TSB t |` cs)) |` cs)) \<sqsubseteq> Rep_TSB (tta (\<lambda>t. Rep_TSB t |` cs)) 
+              (cc (Rep_TSB (tta (\<lambda>t. Rep_TSB t |` cs)) |` cs) 
+              (Rep_TSB (tt (\<lambda>t. Rep_TSB t |` cs)) |` cs))) 
+              \<noteq> ((Rep_TSB (tt (\<lambda>t. Rep_TSB t |` cs)) |` cs) 
+              (cc (Rep_TSB (tta (\<lambda>t. Rep_TSB t |` cs)) |` cs) 
+              (Rep_TSB (tt (\<lambda>t. Rep_TSB t |` cs)) |` cs)) 
+              \<sqsubseteq> (Rep_TSB (tta (\<lambda>t. Rep_TSB t |` cs)) |` cs) 
+              (cc (Rep_TSB (tta (\<lambda>t. Rep_TSB t |` cs)) |` cs) 
+              (Rep_TSB (tt (\<lambda>t. Rep_TSB t |` cs)) |` cs)))"
+      then have "cc (Rep_TSB (tta (\<lambda>t. Rep_TSB t |` cs)) |` cs) 
+                  (Rep_TSB (tt (\<lambda>t. Rep_TSB t |` cs)) |` cs) \<notin> cs"
         by force
-      then have "(Rep_TSB (tt (\<lambda>t. Rep_TSB t |` cs)) |` cs) (cc (Rep_TSB (tta (\<lambda>t. Rep_TSB t |` cs)) |` cs) (Rep_TSB (tt (\<lambda>t. Rep_TSB t |` cs)) |` cs)) \<sqsubseteq> (Rep_TSB (tta (\<lambda>t. Rep_TSB t |` cs)) |` cs) (cc (Rep_TSB (tta (\<lambda>t. Rep_TSB t |` cs)) |` cs) (Rep_TSB (tt (\<lambda>t. Rep_TSB t |` cs)) |` cs))"
+      then have "(Rep_TSB (tt (\<lambda>t. Rep_TSB t |` cs)) |` cs) 
+                  (cc (Rep_TSB (tta (\<lambda>t. Rep_TSB t |` cs)) |` cs) 
+                  (Rep_TSB (tt (\<lambda>t. Rep_TSB t |` cs)) |` cs)) 
+                  \<sqsubseteq> (Rep_TSB (tta (\<lambda>t. Rep_TSB t |` cs)) |` cs) 
+                  (cc (Rep_TSB (tta (\<lambda>t. Rep_TSB t |` cs)) |` cs) 
+                  (Rep_TSB (tt (\<lambda>t. Rep_TSB t |` cs)) |` cs))"
         by simp }
     ultimately have ?thesis
       using f3 f1 by meson }
@@ -458,104 +445,57 @@ qed
 
 
 lemma tsbrestrict_cont1[simp]: "cont  (\<lambda>b. ((Rep_TSB b) |` cs))"
-  apply(rule contI2)
-   apply(auto)
-  by (smt below_option_def fun_below_iff is_ub_thelub lub_eq lub_fun po_class.chain_def rep_chain rep_lub restrict_in restrict_out)
+  apply (rule contI2)
+   apply (auto)
+  by (smt below_option_def fun_below_iff is_ub_thelub lub_eq lub_fun po_class.chain_def 
+          rep_chain rep_lub restrict_in restrict_out)
 
 lemma tsbrestrict_cont [simp]: "cont (\<lambda>b. Abs_TSB (Rep_TSB b |` cs))"
-  by (simp add: cont_Abs_TSB)
+  by simp
 
 lemma tsbrestrict_insert : "tsbRestrict cs\<cdot>tb = Abs_TSB (Rep_TSB tb |` cs)"
-  by(simp add: tsbRestrict_def)
+  by (simp add: tsbRestrict_def)
 
 lemma tsbrestrict_rep_eq : "tsb_well tb \<Longrightarrow> tsbRestrict cs\<cdot>(Abs_TSB tb) = Abs_TSB (tb |` cs)"
-  by(simp add: tsbRestrict_def)
+  by (simp add: tsbRestrict_def)
 
 
 lemma tsbrestrict_dom [simp]: "tsbDom\<cdot>(tb \<bar> cs) \<subseteq> cs"
-  by(simp add: tsbrestrict_insert tsbdom_insert)
+  by (simp add: tsbrestrict_insert tsbdom_insert)
 
 lemma tsresrict_dom2 [simp]: assumes "cs \<subseteq> tsbDom\<cdot>tb"
   shows "tsbDom\<cdot>(tb \<bar> cs) = cs"
-  by (metis Abs_TSB_inverse Int_absorb1 assms dom_restrict mem_Collect_eq tsbdom_insert tsbrestrict_insert tsbrestrict_well)
+  by (metis Abs_TSB_inverse Int_absorb1 assms dom_restrict mem_Collect_eq tsbdom_insert 
+            tsbrestrict_insert tsbrestrict_well)
 
 lemma tsresrict_dom3 [simp]: shows "tsbDom\<cdot>(tb \<bar> cs) = tsbDom\<cdot>tb \<inter> cs"
-  by(simp add: tsbrestrict_insert tsbdom_insert)
+  by (simp add: tsbrestrict_insert tsbdom_insert)
 
 
 lemma [simp]: "(tb \<bar> cs1) \<bar> cs2 = tb \<bar> (cs1\<inter>cs2)"
-  by(simp add: tsbrestrict_insert)
+  by (simp add: tsbrestrict_insert)
 
 lemma tsbgetch_restrict [simp]: assumes "c \<in>cs"
   shows "(tb \<bar> cs)  .  c = tb  .  c"
-  by(simp add: tsbgetch_insert tsbrestrict_insert assms)
-
-
-
-
-
-
-
-
+  by (simp add: tsbgetch_insert tsbrestrict_insert assms)
 
 
 
 subsubsection \<open>tsbTickCount\<close>
-
-(*Experimentell ... *)
-
-thm tsbTickCount_def
-
-lemma tsbtickcount_cont[simp]: "cont (\<lambda> tb. if tsbDom\<cdot>tb \<noteq> {} then #\<surd>(SOME ts. ts \<in> ran (Rep_TSB tb)) else \<infinity>)"
-apply(rule contI2)
-apply(rule monofunI)
-  sorry
-    
-lemma tsbtickcount_insert: "tsbTickCount\<cdot>tb = (if tsbDom\<cdot>tb \<noteq> {} then #\<surd>(SOME ts. ts \<in> ran (Rep_TSB tb)) else \<infinity>)"
-  by (simp add: tsbTickCount_def)
-    
-lemma tsbtickcountch_eq1: "\<exists>n. \<forall> c \<in> tsbDom\<cdot>tb . n = #\<surd> (tb . c)"
-  by (metis ts_ex_len tsbdom_insert tsbgetch_insert)
-   
+  
 lemma tstbtickcount_eq2: "\<exists>n. n = #\<surd> SOME ts. ts \<in> ran (Rep_TSB tb)"
   by simp
-    
-lemma tsbtickcountgetch: assumes "c \<in> tsbDom\<cdot>tb"
-  shows "#\<surd>tsb tb = #\<surd> (tb . c)"
-proof -
-  have f0: "tsbDom\<cdot>tb \<noteq> {}"
-    using assms by auto
-
-  have f1:"(Rep_TSB tb\<rightharpoonup>c) \<in> ran (Rep_TSB tb)"
-    by (metis assms domIff option.exhaust_sel ranI tsbdom_insert)
-  have f2: "\<forall> ts \<in> ran (Rep_TSB tb). \<exists> c \<in> tsbDom\<cdot>tb.  ts = (tb . c)"
-    by (smt Abs_cfun_inverse2 domI mem_Collect_eq option.sel ran_def tsbDom_def tsbdom_cont tsbgetch_insert)
-  hence f3: "\<exists>n. \<forall> ts \<in> ran (Rep_TSB tb). #\<surd> ts = n"
-    by (metis ts_ex_len tsbdom_insert tsbgetch_insert)
-  show ?thesis
-    apply (simp add: tsbTickCount_def tsbgetch_insert, simp add: f0) 
-    by (metis f1 f3 someI_ex)
-qed
-  
-
-lemma "cs \<noteq> {} \<Longrightarrow> #\<surd>tsb (tsbLeast cs) = Fin 0"
-apply(simp add: tsbTickCount_def)
-apply(simp add:  tsbLeast_def, simp add: optionLeast_def)
-apply auto
-oops
-
-
-  
 
 lemma tsb_newMap_well[simp]: assumes "c\<in>tsbDom\<cdot>b"
   shows "tsb_well [c \<mapsto> b  .  c]"
-  apply(simp add: tsbgetch_insert)
+  apply (simp add: tsbgetch_insert)
   apply (rule tsb_wellI)
-   apply (metis (mono_tags) Rep_TSB assms dom_def fun_upd_apply mem_Collect_eq option.sel tsb_well_def tsbdom_insert)
-  by auto
+  by (metis (mono_tags) Rep_TSB assms dom_def fun_upd_apply mem_Collect_eq option.sel 
+                        tsb_well_def tsbdom_insert)
 
 lemma tsb_newMap_id[simp]: assumes "{c}=tsbDom\<cdot>b" shows "Abs_TSB [c \<mapsto> b  .  c] = b"
-  by (metis Rep_TSB_inverse assms domIff dom_eq_singleton_conv fun_upd_same option.collapse tsbdom_insert tsbgetch_insert)
+  by (metis Rep_TSB_inverse assms domIff dom_eq_singleton_conv fun_upd_same option.collapse 
+            tsbdom_insert tsbgetch_insert)
 
 lemma tsb_newMap_restrict [simp]: assumes "c\<in>tsbDom\<cdot>b"
   shows "Abs_TSB [c \<mapsto> b  .  c] = b \<bar> {c}"
@@ -567,50 +507,49 @@ proof -
   then show ?thesis
     using f1 by (simp add: tsbgetch_insert tsbrestrict_insert)
 qed
-  
+
 subsubsection \<open>tsbTTake\<close>
-  
-  
+
+
 thm tsbTTake_def
 lemma tsbttake_well[simp]: "tsb_well (\<lambda>c. (c \<in> tsbDom\<cdot>tb)\<leadsto> ((tb  .  c) \<down> n ))"
-  apply(simp add: tsb_well_def)
-  apply rule
-   apply (metis (full_types) Rep_TSB dual_order.trans mem_Collect_eq tsb_well_def tsbdom_insert tsbgetch_insert tsttake_dom)
-  by (metis Rep_TSB mem_Collect_eq tsb_well_def tsbdom_insert tsbgetch_insert)
+  apply (simp add: tsb_well_def)
+  by (metis (full_types) Rep_TSB dual_order.trans mem_Collect_eq tsb_well_def tsbdom_insert 
+                         tsbgetch_insert tsttake_dom)
 
 lemma tsbttake_dom [simp]: "tsbDom\<cdot>(tb \<down> i) = tsbDom\<cdot>tb"
-  by(simp add: tsbTTake_def tsbdom_rep_eq)
+  by (simp add: tsbTTake_def tsbdom_rep_eq)
 
 lemma tsbttake2least: "(tb \<down> 0) = tsbLeast (tsbDom\<cdot>tb)"
-  apply(rule tsb_eq)
-   apply(simp)
+  apply (rule tsb_eq)
+   apply (simp)
   apply simp
-  by(simp add: tsbTTake_def tsbgetch_insert)
+  by (simp add: tsbTTake_def tsbgetch_insert)
 
 lemma [simp]: assumes "c\<in>tsbDom\<cdot>tb"
   shows "tb \<down> 0  .  c = \<bottom>"
-  by(simp add: tsbttake2least assms)
+  by (simp add: tsbttake2least assms)
 
 lemma [simp]: "c \<in> tsbDom\<cdot>tb \<Longrightarrow> ((tb \<down> n)  .  c) = ((tb  .  c) \<down>n)"
-by(simp add: tsbTTake_def tsbgetch_insert)
+by (simp add: tsbTTake_def tsbgetch_insert)
 
 lemma tsbttake_below [simp]: fixes tb:: "'m TSB"
   shows "(tb \<down> i) \<sqsubseteq> tb"
-  by(rule tsb_below, auto)
- 
+  by (rule tsb_below, auto)
+
 
 lemma tsbttake_lub [simp] : fixes tb:: "'m TSB"
   shows "(\<Squnion>i. (tb \<down> i)) = tb"
-    apply(rule tsb_eq)
-    
+  apply (rule tsb_eq)
+
   oops
-    
-  subsubsection \<open>tsbTTakeL\<close>    
+
+  subsubsection \<open>tsbTTakeL\<close>
 
 lemma tsTakel_lub1_getch_eq: assumes "chain Y" and "c \<in> tsbDom\<cdot>tb"
   shows "tsTakeL\<cdot>(Lub Y)\<cdot>(tb  .  c) \<sqsubseteq> (\<Squnion>i::nat. tsTakeL\<cdot>(Y i)\<cdot>(tb  .  c))"
   by (simp add: assms(1) contlub_cfun_arg contlub_cfun_fun)
-    
+
 lemma tsTakel_lub2_getch_eq: assumes "chain Y" and "c \<in> tsbDom\<cdot>(Lub Y)"
   shows "tsTakeL\<cdot>n\<cdot>(Lub Y  .  c) \<sqsubseteq> (\<Squnion>i. tsTakeL\<cdot>n\<cdot>(Y i  .  c))"
 proof -
@@ -619,52 +558,48 @@ proof -
       by (simp add: assms contlub_cfun_arg contlub_cfun_fun)
     then show "tsTakeL\<cdot>n\<cdot>(Lub Y . c) \<sqsubseteq> (\<Squnion>na. tsTakeL\<cdot>n\<cdot>(Y na . c))"
       by simp
-qed    
-    
-    
-lemma tsbttakeL_well [simp]: "tsb_well (\<lambda>c. (c\<in>tsbDom\<cdot>tb) \<leadsto> (tsTakeL\<cdot>n\<cdot>(tb  .  c)))"  
+qed
+
+
+lemma tsbttakeL_well [simp]: "tsb_well (\<lambda>c. (c\<in>tsbDom\<cdot>tb) \<leadsto> (tsTakeL\<cdot>n\<cdot>(tb  .  c)))"
 proof (cases "n \<noteq> \<infinity>")
   case True
-  have f1: "n < \<infinity>" 
+  have f1: "n < \<infinity>"
     by (simp add: True less_le)
   obtain j where f2: "n = Fin j"
   by (metis f1 infI neq_iff)
   thus ?thesis
   apply (simp add: tsb_well_def tsTakeL_def)
-  apply rule
-    apply (metis (no_types, lifting) subset_trans tsbgetch_insert tsdom_ctype_subset tsttake_dom)
-    by (metis ts_ex_len tsbdom_insert tsbgetch_insert)
+  by (metis (no_types, lifting) subset_trans tsbgetch_insert tsdom_ctype_subset tsttake_dom)
 next
   case False
   then show ?thesis
     apply (simp add: tsb_well_def tsTakeL_def)
-    apply rule
-      apply (simp add: tsbgetch_insert)
-      by (metis ts_ex_len tsbdom_insert tsbgetch_insert)
+    by (simp add: tsbgetch_insert)
   qed
-    
+
 lemma tsbttakeL_dom [simp]: "tsbDom\<cdot>(tsbTTakeL i tb) = tsbDom\<cdot>tb"
   by (simp add: tsbTTakeL_def tsbdom_rep_eq)
-    
+
 lemma tsbttakeL_least: "tsbTTakeL (Fin 0) tb = tsbLeast (tsbDom\<cdot>tb)"
   apply (rule tsb_eq, simp_all)
-  by(simp add: tsbTTakeL_def tsbgetch_insert)
-    
+  by (simp add: tsbTTakeL_def tsbgetch_insert)
+
 lemma tsbttakeL_inf [simp]: "(tsbTTakeL \<infinity> tb) = tb"
   apply (simp add: tsbTTakeL_def)
   apply (simp only: tstakeL_inf)
     by (metis (no_types) tsbgetch_eq2)
-  
+
 lemma tsbttakeL_least_getch [simp]: assumes "c \<in> tsbDom\<cdot>tb"
   shows "(tsbTTakeL (Fin 0) tb) . c = \<bottom>"
   by (metis assms tsbleast_getch tsbttakeL_least)
 
-    
+
 lemma tsbttakeL_getch [simp]: assumes "c \<in> tsbDom\<cdot>tb"
   shows "((tsbTTakeL n tb) . c) = tsTakeL\<cdot>n\<cdot>(tb . c)"
 proof (cases "n \<noteq> \<infinity>")
   case True
-  have f1: "n < \<infinity>" 
+  have f1: "n < \<infinity>"
       by (simp add: True less_le)
   obtain j where f2: "n = Fin j"
   by (metis f1 infI neq_iff)
@@ -678,34 +613,10 @@ next
     apply (simp add: tsbTTakeL_def)
     using False by auto
 qed
-  
+
 lemma tsbttakeL_below [simp]: "(tsbTTakeL n tb) \<sqsubseteq> tb"
   by (rule tsb_below, auto)
-    
-lemma tsbttakeL_len: assumes "tsbDom\<cdot>tb \<noteq> {}"
- shows "#\<surd>tsb (tsbTTakeL (n) tb) = min (#\<surd>tsb tb) (n)"
-proof (cases "n \<noteq> \<infinity>")
-  case True
-  have f1: "n < \<infinity>" 
-    by (simp add: True less_le)
-  obtain j where f2: "n = Fin j"
-    by (metis f1 infI neq_iff)
-  obtain c where f3: "c \<in> tsbDom\<cdot>tb"
-    using assms by blast
-  have f4: "#\<surd>tsb (tsbTTakeL (n) tb) = #\<surd> (tsbTTakeL (n) tb) . c"
-    by (rule tsbtickcountgetch, simp add: f3)
-  have f5: "(tsbTTakeL (n) tb) . c = tsTakeL\<cdot>n\<cdot>(tb . c)"
-    by (simp add: f3)
-  have f6: "#\<surd> (tb . c) = #\<surd>tsb tb"
-    by (subst tsbtickcountgetch, simp_all add: f3)
-  then show ?thesis
-    by (simp add: f4 f5)
-next
-  case False
-  then show ?thesis
-    by simp
-qed
-  
+
 lemma tsbttake_mono2 [simp]: "monofun (\<lambda> tb. tsbTTakeL n tb)"
   apply (rule monofunI)
   apply (rule tsb_below)
@@ -713,9 +624,9 @@ lemma tsbttake_mono2 [simp]: "monofun (\<lambda> tb. tsbTTakeL n tb)"
   apply (subst tsbttakeL_getch, simp)
     apply (subst tsbttakeL_getch, simp add: tsbdom_below)
   by (simp add: monofun_cfun_arg monofun_cfun_fun)
-    
 
-  
+
+
 lemma tsbttake_mono1 [simp]: "\<And> tb. monofun (\<lambda> n. tsbTTakeL n tb)"
   apply (rule monofunI)
   apply (rule tsb_below)
@@ -723,7 +634,7 @@ lemma tsbttake_mono1 [simp]: "\<And> tb. monofun (\<lambda> n. tsbTTakeL n tb)"
    apply (subst tsbttakeL_getch, simp)
    apply (subst tsbttakeL_getch, simp add: tsbdom_below)
   by (simp add: monofun_cfun_arg monofun_cfun_fun)
-    
+
 lemma tsbttake_chain1: assumes "chain Y"
   shows "chain (\<lambda>i::nat. tsbTTakeL (Y i) tb)"
 proof -
@@ -733,8 +644,8 @@ proof -
       apply (rule chainI)
       using assms po_class.chainE by blast
 qed
-    
-  
+
+
 lemma tsbttake_cont1_pre: assumes "chain Y"
   shows "tsbTTakeL (\<Squnion>i. Y i) tb \<sqsubseteq> (\<Squnion>i::nat. tsbTTakeL (Y i) tb)"
 proof -
@@ -746,13 +657,13 @@ proof -
      apply (subst tsbdom_lub, simp_all add: assms)
      apply (simp only: tsbttake_chain1 assms)
        apply (simp add: f1 assms)
-       by (simp add: tsTakel_lub1_getch_eq assms) 
+       by (simp add: tsTakel_lub1_getch_eq assms)
 qed
-  
+
 lemma tsbttake_cont1 [simp]: "\<And>tb. cont (\<lambda> n. tsbTTakeL n tb)"
   apply (rule contI2)
-    by (simp_all add: tsbttake_cont1_pre)    
- 
+    by (simp_all add: tsbttake_cont1_pre)
+
 lemma tsbttake_cont2_pre: assumes "chain Y"
   shows "tsbTTakeL n (\<Squnion>i. Y i) \<sqsubseteq> (\<Squnion>i. tsbTTakeL n (Y i))"
 proof -
@@ -767,109 +678,47 @@ proof -
       apply (simp only: f1, simp add: assms)
       by (simp add: tsTakel_lub2_getch_eq assms)
 qed
-  
+
 lemma tsbttake_cont2 [simp]: "\<And>n. cont (\<lambda> tb. tsbTTakeL n tb)"
   apply (rule contI2)
    by (simp_all add: tsbttake_cont2_pre)
-    
+
 subsubsection \<open>tsbUnion\<close>
 
-(* ----------------------------------------------------------------------- 
-  subsection \<open>tsbUnion \<close>
- ----------------------------------------------------------------------- *)
-
-(* tsbUnion wurde geschrieben bevor alle channels gleich viele ticks haben müssen. 
-    Daher viel anpassen nötig *)
-
-declare [[show_types]]
-
-
-lemma tsbunion_well_pre1[simp]: assumes "tsb_well b1" and "tsb_well b2" 
-                           and "\<forall>c1 \<in> dom b1. \<forall> c2 \<in> dom b2.  #\<surd>(b1\<rightharpoonup>c1) = #\<surd>(b2\<rightharpoonup>c2)"
-  shows "tsb_well (b1 ++ b2)"        
+  
+lemma tsbunion_well [simp]: assumes "tsb_well b1" and "tsb_well b2"
+  shows "tsb_well (b1 ++ b2)"
 proof -
   have "(\<forall>c\<in>dom b2 \<union> dom b1. tsDom\<cdot>b1 ++ b2\<rightharpoonup>c \<subseteq> ctype c)"
-    by (metis (full_types) Un_iff assms(1) assms(2) map_add_dom_app_simps(1) 
+    by (metis (full_types) Un_iff assms(1) assms(2) map_add_dom_app_simps(1)
                map_add_dom_app_simps(3) tsb_well_def)
-  moreover have "(\<exists>n::lnat. \<forall>c\<in>dom b2 \<union> dom b1. #\<surd> b1 ++ b2\<rightharpoonup>c = n)"
-    by (metis (no_types, lifting) UnE assms(1) assms(2) assms(3) map_add_dom_app_simps(1) 
-              map_add_dom_app_simps(3) tsb_well_def)
-  ultimately show ?thesis
+  thus ?thesis
     using tsb_well_def by blast
 qed
-  
-    
-lemma tsbunion_well [simp]: 
-  shows "tsb_well ((Rep_TSB (tsbTTakeL (#\<surd>tsb tb2) tb1)) ++ (Rep_TSB (tsbTTakeL (#\<surd>tsb tb1) tb2)))"
-proof (cases "tsbDom\<cdot>tb1 = {} \<or> tsbDom\<cdot>tb2 = {}")
-  case True
-  then show ?thesis
-     by (metis Rep_TSB True empty_iff mem_Collect_eq tsbdom_insert tsbttakeL_dom tsbunion_well_pre1)
-next
-  case False
-  have f0: "tsbDom\<cdot>tb1 \<noteq> {} \<and> tsbDom\<cdot>tb2 \<noteq> {}"
-    using False by auto
-  then show ?thesis
-    proof (cases "(#\<surd>tsb tb2) < (#\<surd>tsb tb1)")
-      case True
-      hence "#\<surd>tsb (tsbTTakeL (#\<surd>tsb tb2) tb1) = (#\<surd>tsb tb2)"
-        by (simp add: f0 min_absorb2 tsbttakeL_len)
-      thus ?thesis
-        by (metis (no_types, lifting) Rep_TSB True f0 mem_Collect_eq min.strict_order_iff 
-            tsbdom_insert tsbgetch_insert tsbtickcountgetch tsbttakeL_len tsbunion_well_pre1)
-    next
-      case False
-      hence "#\<surd>tsb (tsbTTakeL (#\<surd>tsb tb1) tb2) = (#\<surd>tsb tb1)"
-        by (simp add: f0 min_absorb2 tsbttakeL_len)
-      then show ?thesis
-        by (metis (no_types, lifting) Rep_TSB f0 mem_Collect_eq min.commute 
-                  tsbdom_insert tsbgetch_insert tsbtickcountgetch tsbttakeL_len tsbunion_well_pre1)  
-    qed
-qed
-  
 
 (* helper function for continuity proof *)
-lemma tsbunion_contL[simp]: "\<And> b2. cont (\<lambda>b1. (Rep_TSB b1) ++ (Rep_TSB b2))"
+lemma tsbunion_contL[simp]: "cont (\<lambda>b1. (Rep_TSB b1) ++ (Rep_TSB b2))"
   using cont_compose part_add_contL rep_tsb_cont by blast
-    
-lemma tsbunion_contL1 [simp]: "\<And> tb2. cont (\<lambda> tb1. (Rep_TSB (tsbTTakeL (#\<surd>tsb tb2) tb1)) ++ (Rep_TSB (tsbTTakeL (#\<surd>tsb tb1) tb2)))"
-(* proof -
-  have f0: "\<And> tb2. cont (\<lambda> tb1. (Rep_TSB (tsbTTakeL (#\<surd>tsb tb2) tb1)))"
-    by (simp add: cont_Rep_TSB)
-  moreover
-  have f1: "\<And> tb2. cont (\<lambda> tb1. (Rep_TSB (tsbTTakeL (#\<surd>tsb tb1) tb2)))"
-    sorry
-  ultimately
-  show "\<And> tb2. cont (\<lambda> tb1. (Rep_TSB (tsbTTakeL (#\<surd>tsb tb2) tb1)) ++ (Rep_TSB (tsbTTakeL (#\<surd>tsb tb1) tb2)))"
-    apply (simp add: cont_compose part_add_contL f0 f1)
-    using cont_compose part_add_contL by blast
-    *) sorry
 
 (* helper function for continuity proof *)
-lemma tsbunion_contR[simp]: "\<And> b1. cont (\<lambda>b2. (Rep_TSB b1) ++ (Rep_TSB b2))"
+lemma tsbunion_contR[simp]: "cont (\<lambda>b2. (Rep_TSB b1) ++ (Rep_TSB b2))"
   using cont_compose part_add_contR rep_tsb_cont by blast
-    
-lemma tsbunion_contR1 [simp]: "\<And> tb1. cont (\<lambda> tb2. (Rep_TSB (tsbTTakeL (#\<surd>tsb tb2) tb1)) ++ (Rep_TSB (tsbTTakeL (#\<surd>tsb tb1) tb2)))"
-  sorry
 
 (* sbUnion is an coninuous function *)
-lemma tsbunion_cont[simp]:
-  shows "cont (\<lambda> tb1. \<Lambda> tb2. Abs_TSB ((Rep_TSB (tsbTTakeL (#\<surd>tsb tb2) tb1)) ++ (Rep_TSB (tsbTTakeL (#\<surd>tsb tb1) tb2))) )"
+lemma tsbunion_cont[simp]: "cont (\<lambda> b1. \<Lambda> b2.(Abs_TSB (Rep_TSB b1 ++ Rep_TSB b2)))"
   by(simp add: cont2cont_LAM cont_Abs_TSB)
     
-(*
 (* insert rule for sbUnion *)
-lemma tsbunion_insert: assumes "#\<surd>tsb tb1 = #\<surd>tsb tb2"
-shows "(tb1 \<uplus> tb2) = (Abs_TSB (Rep_TSB tb1 ++ Rep_TSB tb2))"
-  apply (simp add: tsbUnion_def)
-    oops
+lemma tsbunion_insert: "(tb1 \<uplus> tb2) = (Abs_TSB (Rep_TSB tb1 ++ Rep_TSB tb2))"
+  by(simp add: tsbUnion_def)
 
 (* if all channels in b1 are also in b2 the union produces b2 *)
 lemma tsbunion_idL [simp]: assumes "tsbDom\<cdot>tb1\<subseteq>tsbDom\<cdot>tb2" shows "tb1 \<uplus> tb2 = tb2"
   by (metis Rep_TSB_inverse assms part_add_id tsbdom_insert tsbunion_insert)
 
 lemma tsbunion_idR [simp]: "b \<uplus> (tsbLeast {}) = b"
-  by (metis Int_absorb1 Rep_TSB_inverse empty_subsetI map_add_comm part_add_id tsbdom_insert tsbleast_tsdom tsbunion_insert)
+  by (metis Int_absorb1 Rep_TSB_inverse empty_subsetI map_add_comm part_add_id tsbdom_insert 
+            tsbleast_tsdom tsbunion_insert)
 
 (* if b1 and b2 have no common channels, sbUnion is commutative *)
 lemma tsbunion_commutative: assumes "tsbDom\<cdot>b1 \<inter> tsbDom\<cdot>b2 = {}"
@@ -891,7 +740,8 @@ lemma tsbunion_getchL [simp]: assumes "c\<notin>tsbDom\<cdot>b2"
 lemma tsbunion_restrict3 [simp]: assumes "(tsbDom\<cdot>y)\<inter>(tsbDom\<cdot>x) = {}" 
   shows "(x\<uplus>y) \<bar> tsbDom\<cdot>x = x"
   apply(simp add: tsbunion_insert tsbdom_insert)
-  by (metis Abs_TSB_inverse Rep_TSB Rep_TSB_inverse assms map_add_comm map_union_restrict2 mem_Collect_eq tsbdom_insert tsbrestrict_insert tsbunion_well)
+  by (metis Abs_TSB_inverse Rep_TSB Rep_TSB_inverse assms map_add_comm map_union_restrict2 
+            mem_Collect_eq tsbdom_insert tsbrestrict_insert tsbunion_well)
 
 lemma tsbunion_restrict2 [simp]:"(x\<uplus>y) \<bar> tsbDom\<cdot>y = y"
   by(simp add: tsbunion_insert tsbdom_insert tsbrestrict_insert)
@@ -903,14 +753,7 @@ lemma tsbunion_restrict [simp]: assumes "(tsbDom\<cdot>y)\<inter>cs2 = {}"
 lemma tsbunion_dom [simp]: "tsbDom\<cdot>(tb1 \<uplus> tb2) = tsbDom\<cdot>tb1 \<union> tsbDom\<cdot>tb2"
   by(simp add: tsbdom_insert tsbunion_insert Un_commute)
 
-*)
 
-
-
-    
-
-
- 
 
 
 
@@ -922,11 +765,11 @@ lemma tsbunion_dom [simp]: "tsbDom\<cdot>(tb1 \<uplus> tb2) = tsbDom\<cdot>tb1 \
 
 
 definition tsb_fin_well :: "(channel \<rightharpoonup> 'm tstream) \<Rightarrow> bool" where
-"tsb_fin_well f \<equiv> (\<forall>c \<in> dom f. tsDom\<cdot>(f\<rightharpoonup>c) \<subseteq> ctype c) 
+"tsb_fin_well f \<equiv> (\<forall>c \<in> dom f. tsDom\<cdot>(f\<rightharpoonup>c) \<subseteq> ctype c)
            \<and> (\<exists>n. \<forall>c \<in> dom f.  #\<surd>(f\<rightharpoonup>c) = Fin n)"
 
 lemma tsb_fin_exists [simp]: "tsb_fin_well empty"
-  by(simp add: tsb_fin_well_def)
+  by (simp add: tsb_fin_well_def)
 
 typedef ('m :: message) TSB_fin = "{b :: channel \<rightharpoonup> 'm tstream . tsb_fin_well b }"
   using tsb_fin_exists by blast
@@ -940,27 +783,27 @@ typedef ('m :: message) TSB_fin = "{b :: channel \<rightharpoonup> 'm tstream . 
   section \<open>TSB-inf\<close>
 (* ----------------------------------------------------------------------- *)
 
-    
+
   subsection \<open>Definitions on TSB-inf \<close>
 (* ----------------------------------------------------------------------- *)
 
 definition tsb_inf_well :: "(channel \<rightharpoonup> 'm tstream) \<Rightarrow> bool" where
-"tsb_inf_well f \<equiv> (\<forall>c \<in> dom f. tsDom\<cdot>(f\<rightharpoonup>c) \<subseteq> ctype c) 
+"tsb_inf_well f \<equiv> (\<forall>c \<in> dom f. tsDom\<cdot>(f\<rightharpoonup>c) \<subseteq> ctype c)
                 \<and> (\<forall>c \<in> dom f. #\<surd>(f\<rightharpoonup>c) = \<infinity>)"
 
 
 lemma tsb_inf_exists [simp]: "tsb_inf_well empty"
-  by(simp add: tsb_inf_well_def)
+  by (simp add: tsb_inf_well_def)
 
 lemma tsb_inf_adm[simp]: "adm (\<lambda>x. \<forall>c\<in>dom x. #\<surd> x\<rightharpoonup>c = \<infinity>)"
-  apply(rule admI)
+  apply (rule admI)
   apply rule+
   by (simp add: contlub_cfun_arg part_dom_lub part_the_chain part_the_lub)
 
 
 cpodef ('m :: message) TSB_inf = "{b :: channel \<rightharpoonup> 'm tstream . tsb_inf_well b }"
    using tsb_inf_exists apply blast
-  by(simp add: tsb_inf_well_def)
+  by (simp add: tsb_inf_well_def)
 
 setup_lifting type_definition_TSB_inf
 
@@ -978,7 +821,7 @@ abbreviation tsbigetch_abbrv :: "'m TSB_inf \<Rightarrow> channel \<Rightarrow> 
 "tbi  .  c \<equiv> tsbiGetCh\<cdot>tbi\<cdot>c"
 
 
-definition tsbiUnion :: "'m TSB_inf \<rightarrow> 'm TSB_inf \<rightarrow> 'm TSB_inf"  where 
+definition tsbiUnion :: "'m TSB_inf \<rightarrow> 'm TSB_inf \<rightarrow> 'm TSB_inf"  where
 "tsbiUnion \<equiv> \<Lambda> tb1 tb2 . Abs_TSB_inf ((Rep_TSB_inf tb1) ++ (Rep_TSB_inf tb2))"
 
 abbreviation tsbiUnion_abbrv :: "'m TSB_inf \<Rightarrow> 'm TSB_inf \<Rightarrow> 'm TSB_inf" (infixl "\<uplus>" 100) where
@@ -1015,7 +858,7 @@ definition tsbInf2tsb :: "'m TSB_inf \<rightarrow> 'm TSB" where
 
   subsection \<open>lemmas on TSB-inf \<close>
 (* ----------------------------------------------------------------------- *)
-    
+
 lemma [simp]: "tsb_inf_well (Rep_TSB_inf x)"
   using Rep_TSB_inf by blast
 
@@ -1044,7 +887,7 @@ lemma tsbi_blow_eq [simp]:  fixes x y :: "'m TSB_inf"
 qed
 
 instance TSB_inf :: ( message ) discrete_cpo
-  apply(intro_classes)
+  apply (intro_classes)
   using tsbi_blow_eq by blast
 
 
@@ -1059,13 +902,13 @@ lemma tsbi_option_below [simp]:
   assumes "x\<sqsubseteq>y"
   shows "x = y"
   using assms below_option_def fun_below_iff by fastforce
-  
 
-lemma tsbi_option_chain_max_in [simp]: 
+
+lemma tsbi_option_chain_max_in [simp]:
   fixes Y:: "nat \<Rightarrow> ('a TSB_inf \<rightharpoonup> 'b TSB_inf)"
   assumes "chain Y"
   shows "max_in_chain 0 Y"
-  apply(rule max_in_chainI)
+  apply (rule max_in_chainI)
 proof -
   fix j :: nat
   have f1: "\<forall>f t. (\<not> chain f) \<or> chain (\<lambda>n. f n\<rightharpoonup>(t::'a TSB_inf)::'b TSB_inf)"
@@ -1078,9 +921,9 @@ proof -
   then show "Y 0 = Y j"
     using f2 f1 by (metis assms is_ub_thelub part_dom_eq1)
 qed
-  
 
-lemma tsbi_option_chain_finite [simp]: 
+
+lemma tsbi_option_chain_finite [simp]:
   fixes Y:: "nat \<Rightarrow> ('a TSB_inf \<rightharpoonup> 'b TSB_inf)"
   assumes "chain Y"
   shows "finite_chain Y"
@@ -1090,28 +933,28 @@ lemma tsbi_option_chain_finite [simp]:
 lemma tsbi_option_adm [simp]:
   fixes g:: "('a TSB_inf \<rightharpoonup> 'b TSB_inf) \<Rightarrow> bool"
   shows "adm g"
-  apply(rule admI)
+  apply (rule admI)
   by (metis l42 tsbi_option_chain_finite)
 
 
 
 
 subsubsection \<open>tsbiDom\<close>
-  
+
 thm tsbiDom_def
 
 lemma tsbidom_insert: "tsbiDom\<cdot>x = dom (Rep_TSB_inf x)"
-  by(simp add: tsbiDom_def)
+  by (simp add: tsbiDom_def)
 
 lemma tsbidom_rep_eq: "tsb_inf_well tbi \<Longrightarrow> tsbiDom\<cdot>(Abs_TSB_inf tbi) = dom tbi"
-by(simp add: tsbidom_insert)
+by (simp add: tsbidom_insert)
 
 
 lemma [simp]: "tsb_inf_well (\<lambda>c.(c\<in>cs) \<leadsto> tsInfTick)"
-by(simp add: tsb_inf_well_def)
+by (simp add: tsb_inf_well_def)
 
 lemma tsbiLeast_dom [simp]: "tsbiDom\<cdot>(Abs_TSB_inf (\<lambda>c.(c\<in>cs) \<leadsto> tsInfTick)) = cs"
-by(simp add: tsbiDom_def)
+by (simp add: tsbiDom_def)
 
 lemma tsbi_dom_ex[simp]: "\<exists>tbi. tsbiDom\<cdot>tbi = cs"
 using tsbiLeast_dom by blast
@@ -1121,7 +964,7 @@ using tsbi_dom_ex tsbidom_insert by fastforce
 
 
 lemma tsbi_ex[simp]: "TSBi cs \<noteq> {}"
-by(simp add: TSBi_def)
+by (simp add: TSBi_def)
 
 
 subsubsection \<open>tsbiGetCh\<close>
@@ -1129,18 +972,18 @@ subsubsection \<open>tsbiGetCh\<close>
 thm tsbiGetCh_def
 
 lemma tsbigetch_insert: "tbi  .  c = (Rep_TSB_inf tbi) \<rightharpoonup> c"
-by(simp add: tsbiGetCh_def)
+by (simp add: tsbiGetCh_def)
 
 lemma tsbigetch_rep_eq: "tsb_inf_well tbi \<Longrightarrow> (Abs_TSB_inf tbi)  .  c = tbi \<rightharpoonup> c"
-by(simp add: tsbiGetCh_def)
+by (simp add: tsbiGetCh_def)
 
 
-lemma tsbi_getch_inf [simp]: 
+lemma tsbi_getch_inf [simp]:
   shows "c\<in>tsbiDom\<cdot>tbi \<Longrightarrow> #\<surd> tbi . c = \<infinity>"
-  by(simp add: tsbiGetCh_def tsbiDom_def)
+  by (simp add: tsbiGetCh_def tsbiDom_def)
 
 lemma tsbi_getch_type[simp]: "c\<in>tsbiDom\<cdot>tbi \<Longrightarrow> tsDom\<cdot>(tbi  .  c) \<subseteq> ctype c"
-apply(simp add: tsbiGetCh_def)
+apply (simp add: tsbiGetCh_def)
 using tsb_inf_well_def tsbidom_insert by fastforce
 
 
@@ -1160,7 +1003,7 @@ subsubsection \<open>tsbiUnion\<close>
 (* tsbUnion produces a welltyped partial-function *)
 lemma tsbiunion_well[simp]: assumes "tsb_inf_well b1" and "tsb_inf_well b2"
   shows "tsb_inf_well (b1 ++ b2)"
-  apply(simp add: tsb_inf_well_def)
+  apply (simp add: tsb_inf_well_def)
   apply (rule, rule)
    apply (metis (no_types, lifting) Un_iff assms(1) assms(2) map_add_dom_app_simps(1) map_add_dom_app_simps(3) tsb_inf_well_def)
   apply rule
@@ -1169,7 +1012,7 @@ lemma tsbiunion_well[simp]: assumes "tsb_inf_well b1" and "tsb_inf_well b2"
 
 (* insert rule for sbUnion *)
 lemma tsbiunion_insert: "(tb1 \<uplus> tb2) = (Abs_TSB_inf (Rep_TSB_inf tb1 ++ Rep_TSB_inf tb2))"
-  by(simp add: tsbiUnion_def)
+  by (simp add: tsbiUnion_def)
 
 (* if all channels in b1 are also in b2 the union produces b2 *)
 lemma tsbiunion_idL:  "tsbiDom\<cdot>tb1\<subseteq>tsbiDom\<cdot>tb2 \<Longrightarrow> tb1 \<uplus> tb2 = tb2"
@@ -1177,26 +1020,26 @@ lemma tsbiunion_idL:  "tsbiDom\<cdot>tb1\<subseteq>tsbiDom\<cdot>tb2 \<Longright
 
 (* if b1 and b2 have no common channels, sbUnion is commutative *)
 lemma tsbiunion_commutative: "tsbiDom\<cdot>b1 \<inter> tsbiDom\<cdot>b2 = {} \<Longrightarrow> b1\<uplus>b2 = b2\<uplus>b1"
-  apply(simp add: tsbiunion_insert)
+  apply (simp add: tsbiunion_insert)
   by (metis map_add_comm tsbidom_insert)
 
 
 (* the second argument has priority in sbUnion *)
 lemma tsbiunion_getchR [simp]:
   shows "c\<in>tsbiDom\<cdot>b2 \<Longrightarrow> b1\<uplus>b2  .  c = b2  .  c"
-  apply(simp add: tsbiunion_insert tsbiGetCh_def )
+  apply (simp add: tsbiunion_insert tsbiGetCh_def )
   by (simp add: map_add_dom_app_simps(1) tsbidom_insert)
 
 lemma tsbiunion_getchL [simp]: "c\<notin>tsbiDom\<cdot>b2 \<Longrightarrow> b1\<uplus>b2  .  c = b1  .  c"
-  apply(simp add: tsbiunion_insert tsbiGetCh_def)
+  apply (simp add: tsbiunion_insert tsbiGetCh_def)
   by (metis map_add_dom_app_simps(3) tsbidom_insert)
 
 lemma tsbiunion_dom [simp]: "tsbiDom\<cdot>(tb1 \<uplus> tb2) = tsbiDom\<cdot>tb1 \<union> tsbiDom\<cdot>tb2"
-  by(simp add: tsbidom_insert tsbiunion_insert Un_commute)
+  by (simp add: tsbidom_insert tsbiunion_insert Un_commute)
 
 lemma tsbiunion_assoc [simp]: fixes x y z :: "'m TSB_inf"
   shows "(x \<uplus> y) \<uplus> z = x \<uplus> (y \<uplus> z)"
-by(simp add: tsbiunion_insert)
+by (simp add: tsbiunion_insert)
 
 
 
@@ -1204,44 +1047,44 @@ by(simp add: tsbiunion_insert)
 
 
 subsubsection \<open>tsbiRes\<close>
-  
+
 lemma [simp]: "tsb_inf_well (Rep_TSB_inf b |` cs)"
-  apply(simp add: tsb_inf_well_def)
+  apply (simp add: tsb_inf_well_def)
   by (metis IntD1 Rep_TSB_inf mem_Collect_eq tsb_inf_well_def)
 
 lemma tsbirestrict_insert: "tbi \<bar> cs = Abs_TSB_inf (Rep_TSB_inf tbi |` cs)"
-  by(simp add: tsbiRestrict_def)
+  by (simp add: tsbiRestrict_def)
 
 lemma tsbirestrict_dom [simp]: "tsbiDom\<cdot>(tb \<bar> cs) \<subseteq> cs"
-  by(simp add: tsbiRestrict_def tsbidom_insert)
+  by (simp add: tsbiRestrict_def tsbidom_insert)
 
 lemma tsbiresrict_dom2 [simp]: "cs \<subseteq> tsbiDom\<cdot>tb \<Longrightarrow> tsbiDom\<cdot>(tb \<bar> cs) = cs"
-  apply(simp add: tsbidom_insert tsbiRestrict_def)
+  apply (simp add: tsbidom_insert tsbiRestrict_def)
   by blast
 
 lemma tsbirestrict_dom3: "tsbiDom\<cdot>(tb \<bar> cs) = tsbiDom\<cdot>tb \<inter> cs"
-  by(simp add: tsbidom_insert tsbiRestrict_def)
+  by (simp add: tsbidom_insert tsbiRestrict_def)
 
 lemma [simp]: fixes tb :: "'m TSB_inf"
   shows "(tb \<bar> cs1) \<bar> cs2 = tb \<bar> (cs1\<inter>cs2)"
-  by(simp add: tsbiRestrict_def)
+  by (simp add: tsbiRestrict_def)
 
 lemma tsbirestrict_dom2 [simp]: "tsbiDom\<cdot>(tb \<bar> cs) = cs \<Longrightarrow> cs \<subseteq> tsbiDom\<cdot>tb"
-  by(auto simp add: tsbidom_insert tsbiRestrict_def)
+  by (auto simp add: tsbidom_insert tsbiRestrict_def)
 
-lemma tsbiRestrict_getch [simp]:  "c \<in> cs \<Longrightarrow> tbi \<bar> cs . c   = tbi . c " 
+lemma tsbiRestrict_getch [simp]:  "c \<in> cs \<Longrightarrow> tbi \<bar> cs . c   = tbi . c "
 by (simp add: tsbirestrict_insert tsbiGetCh_def)
 
 
 lemma tsbiunion_restrict3 [simp]: "(tsbiDom\<cdot>y)\<inter>(tsbiDom\<cdot>x) = {} \<Longrightarrow> (x\<uplus>y) \<bar> tsbiDom\<cdot>x = x"
-  apply(simp add: tsbidom_insert tsbiRestrict_def tsbiunion_insert)
+  apply (simp add: tsbidom_insert tsbiRestrict_def tsbiunion_insert)
   by (metis Int_absorb Rep_TSB_inf_inverse map_union_restrict2 restrict_restrict)
 
 lemma tsbiunion_restrict2 [simp]:"(x\<uplus>y) \<bar> tsbiDom\<cdot>y = y"
-  by(simp add: tsbiunion_insert tsbidom_insert tsbiRestrict_def)
+  by (simp add: tsbiunion_insert tsbidom_insert tsbiRestrict_def)
 
 lemma tsbiunion_restrict [simp]:"(tsbiDom\<cdot>y)\<inter>cs2 = {} \<Longrightarrow> (x\<uplus>y) \<bar> cs2 = x \<bar> cs2"
-  by(simp add: tsbiunion_insert tsbirestrict_insert tsbiDom_def)
+  by (simp add: tsbiunion_insert tsbirestrict_insert tsbiDom_def)
 
 
 
@@ -1254,10 +1097,10 @@ lemma tsbiunion_restrict [simp]:"(tsbiDom\<cdot>y)\<inter>cs2 = {} \<Longrightar
 
 
 subsubsection \<open>tsbiTTake\<close>
-  
+
 thm tsbiTTake_def
 lemma tsbittake_well[simp]: "tsb_well (\<lambda>c. (c \<in> tsbiDom\<cdot>tbi)\<leadsto>tbi . c \<down> n )"
-  apply(rule tsb_wellI)
+  apply (rule tsb_wellI)
    apply simp
    apply (meson order.trans tsbi_getch_type tsttake_dom)
   by (simp add: tsbiGetCh_def tsbidom_insert)
@@ -1265,20 +1108,20 @@ lemma tsbittake_well[simp]: "tsb_well (\<lambda>c. (c \<in> tsbiDom\<cdot>tbi)\<
 
 lemma tsbittake_getch [simp]: fixes tsbi:: "'m TSB_inf"
   shows "c\<in>tsbiDom\<cdot>tsbi \<Longrightarrow> tsbi \<down> n  .  c = tsbi . c \<down>n"
-by(simp add: tsbiTTake_def tsbgetch_insert)
+by (simp add: tsbiTTake_def tsbgetch_insert)
 
 lemma tsbiGetCh_rep_eq: "tsb_inf_well tbi \<Longrightarrow> (Abs_TSB_inf tbi)  .  c = tbi \<rightharpoonup> c "
-by(simp add: tsbiGetCh_def)
+by (simp add: tsbiGetCh_def)
 
 
 lemma [simp]: "tsbDom\<cdot>(tbi \<down> n) = tsbiDom\<cdot>tbi"
-by(simp add: tsbiTTake_def tsbdom_insert)
+by (simp add: tsbiTTake_def tsbdom_insert)
 
 
 lemma tsbiTtake_chain [simp]: fixes tbi :: "'a TSB_inf"
   shows "chain (\<lambda>i. tbi \<down> i)"
-  apply(rule chainI)
-  apply(rule tsb_below)
+  apply (rule chainI)
+  apply (rule tsb_below)
    apply simp
   by simp
 
@@ -1294,22 +1137,22 @@ subsubsection \<open>tsb2tsbInf\<close>
 thm tsb2tsbInf_def
 
 lemma [simp]: "tsb_inf_well (\<lambda>c. (c\<in>tsbDom\<cdot>tb)\<leadsto>(tb  .  c) \<bullet> tsInfTick)"
-  by(simp add: tsb_inf_well_def tsbgetch_insert)
+  by (simp add: tsb_inf_well_def tsbgetch_insert)
 
 lemma tsb2tsbInf_dom [simp]: "tsbiDom\<cdot>(tsb2tsbInf tb) = tsbDom\<cdot>tb"
-  by(simp add: tsb2tsbInf_def tsbidom_insert)
+  by (simp add: tsb2tsbInf_def tsbidom_insert)
 
 lemma rep_tsbi_tsb_well [simp]: "tsb_well (Rep_TSB_inf tbi)"
   using Rep_TSB_inf tsb_inf_well_def tsb_well_def by fastforce
 
 lemma tsbinf2tsb_insert: "tsbInf2tsb\<cdot>tbi = Abs_TSB (Rep_TSB_inf tbi)"
-  by(simp add: tsbInf2tsb_def)
+  by (simp add: tsbInf2tsb_def)
 
 lemma [simp]: "tsbDom\<cdot>(tsbInf2tsb\<cdot>tbi) =tsbiDom\<cdot>tbi"
-  by(simp add: tsbdom_insert tsbinf2tsb_insert tsbidom_insert)
+  by (simp add: tsbdom_insert tsbinf2tsb_insert tsbidom_insert)
 
 lemma tsbInf2tsb_getch [simp]: "tsbInf2tsb\<cdot>tb  . c = tb .  c"
-by(simp add: tsbInf2tsb_def tsbgetch_insert tsbigetch_insert)
+by (simp add: tsbInf2tsb_def tsbgetch_insert tsbigetch_insert)
 
 
 lemma tsbiTtake_Lub [simp]: "(\<Squnion>i. (tb\<down>i)) = tsbInf2tsb\<cdot>tb" (is "?L = ?R")
@@ -1350,13 +1193,13 @@ proof(rule tsb_eq)
   have "tsbDom\<cdot>(b1 \<down> (Suc n)) = tsbDom\<cdot>(b2 \<down> (Suc n))" by (simp add: assms)
   hence dom_eq: "tsbiDom\<cdot>b1 = tsbiDom\<cdot>b2" by simp
   thus "tsbDom\<cdot>(b1 \<down> n) = tsbDom\<cdot>(b2 \<down> n)" by simp
-  
+
   fix c
   assume "c\<in>tsbDom\<cdot>(b1\<down> n)"
   hence c_def: "c\<in>tsbiDom\<cdot>b1" by simp
   hence c_def2: "c\<in>tsbiDom\<cdot>b2" by (simp add: dom_eq)
   hence "b1\<down> (Suc n)  .  c = b2\<down> (Suc n)  .  c" by (simp add: assms)
-  hence "b1  .  c \<down> n = b2  . c \<down> n" using c_def c_def2 by(subst tsSucTake; auto) 
+  hence "b1  .  c \<down> n = b2  . c \<down> n" using c_def c_def2 by (subst tsSucTake; auto)
   thus " b1\<down>n  .  c = b2\<down>n  .  c" by (simp add: c_def dom_eq c_def2)
 qed
 
@@ -1366,6 +1209,92 @@ qed
 end
 
 
+(* OBSOLETE THINGS:
 
+
+definition tsbTickCount :: "'m TSB \<rightarrow> lnat" where
+"tsbTickCount \<equiv>  \<Lambda> tb. if tsbDom\<cdot>tb \<noteq> {} then #\<surd>(SOME ts. ts \<in> ran (Rep_TSB tb)) else \<infinity>"
+
+abbreviation tsbTickCount_abbrv :: "'m TSB \<Rightarrow> lnat "  ("#\<surd>tsb _ ") where
+" #\<surd>tsb tsb \<equiv> tsbTickCount\<cdot>tsb"
+
+
+definition tsbMinTick :: "'m TSB \<Rightarrow> 'm TSB \<Rightarrow> lnat" where
+"tsbMinTick tb1 tb2 \<equiv> lnmin\<cdot>(#\<surd>tsb tb1)\<cdot>(#\<surd>tsb tb2)"
+
+lemma tsb_tick_eq2: assumes "c1\<in>tsbDom\<cdot>f" and "c2\<in>tsbDom\<cdot>f"
+  shows "#\<surd> f . c1 = #\<surd> f . c2"
+  using assms by (simp add: tsbdom_insert tsbgetch_insert tsb_tick_eq)
+
+
+
+
+(*Experimentell ... *)
+
+thm tsbTickCount_def
+
+lemma tsbtickcount_cont[simp]: "cont (\<lambda> tb. if tsbDom\<cdot>tb \<noteq> {} then #\<surd>(SOME ts. 
+                                      ts \<in> ran (Rep_TSB tb)) else \<infinity>)"
+apply (rule contI2)
+apply (rule monofunI)
+  sorry
+
+lemma tsbtickcount_insert: "tsbTickCount\<cdot>tb = (if tsbDom\<cdot>tb \<noteq> {} then #\<surd>(SOME ts. 
+                                                ts \<in> ran (Rep_TSB tb)) else \<infinity>)"
+  by (simp add: tsbTickCount_def)
+
+lemma tsbtickcountch_eq1: "\<exists>n. \<forall> c \<in> tsbDom\<cdot>tb . n = #\<surd> (tb . c)"
+  by (metis ts_ex_len tsbdom_insert tsbgetch_insert)
+
+lemma tsbtickcountgetch: assumes "c \<in> tsbDom\<cdot>tb"
+  shows "#\<surd>tsb tb = #\<surd> (tb . c)"
+proof -
+  have f0: "tsbDom\<cdot>tb \<noteq> {}"
+    using assms by auto
+
+  have f1:"(Rep_TSB tb\<rightharpoonup>c) \<in> ran (Rep_TSB tb)"
+    by (metis assms domIff option.exhaust_sel ranI tsbdom_insert)
+  have f2: "\<forall> ts \<in> ran (Rep_TSB tb). \<exists> c \<in> tsbDom\<cdot>tb.  ts = (tb . c)"
+    by (smt Abs_cfun_inverse2 domI mem_Collect_eq option.sel ran_def tsbDom_def tsbdom_cont 
+            tsbgetch_insert)
+  hence f3: "\<exists>n. \<forall> ts \<in> ran (Rep_TSB tb). #\<surd> ts = n"
+    by (metis ts_ex_len tsbdom_insert tsbgetch_insert)
+  show ?thesis
+    apply (simp add: tsbTickCount_def tsbgetch_insert, simp add: f0)
+    by (metis f1 f3 someI_ex)
+qed
+
+
+lemma "cs \<noteq> {} \<Longrightarrow> #\<surd>tsb (tsbLeast cs) = Fin 0"
+apply (simp add: tsbTickCount_def)
+apply (simp add:  tsbLeast_def, simp add: optionLeast_def)
+apply auto
+oops
+
+lemma tsbttakeL_len: assumes "tsbDom\<cdot>tb \<noteq> {}"
+ shows "#\<surd>tsb (tsbTTakeL (n) tb) = min (#\<surd>tsb tb) (n)"
+proof (cases "n \<noteq> \<infinity>")
+  case True
+  have f1: "n < \<infinity>"
+    by (simp add: True less_le)
+  obtain j where f2: "n = Fin j"
+    by (metis f1 infI neq_iff)
+  obtain c where f3: "c \<in> tsbDom\<cdot>tb"
+    using assms by blast
+  have f4: "#\<surd>tsb (tsbTTakeL (n) tb) = #\<surd> (tsbTTakeL (n) tb) . c"
+    by (rule tsbtickcountgetch, simp add: f3)
+  have f5: "(tsbTTakeL (n) tb) . c = tsTakeL\<cdot>n\<cdot>(tb . c)"
+    by (simp add: f3)
+  have f6: "#\<surd> (tb . c) = #\<surd>tsb tb"
+    by (subst tsbtickcountgetch, simp_all add: f3)
+  then show ?thesis
+    by (simp add: f4 f5)
+next
+  case False
+  then show ?thesis
+    by simp
+qed
+
+*)
 
 
